theories/Util/Quant.v
@@ -1,0 +1,108 @@
+Require Import ExtLib.Data.Prop.
+Require Import MirrorCore.OpenT.
+
+Section quants.
+  Context {typ : Type}.
+  Variable typD : typ -> Type.
+
+  Fixpoint _foralls (ls : list typ)
+  : (OpenT typD ls Prop) -> Prop :=
+    match ls as ls return (OpenT typD ls Prop) -> Prop with
+      | nil => fun P => P HList.Hnil
+      | l :: ls => fun P => forall x : typD l,
+                              _foralls ls (fun z => P (HList.Hcons x z))
+    end.
+
+  Fixpoint _exists (ls : list typ)
+  : (OpenT typD ls Prop) -> Prop :=
+    match ls as ls return (OpenT typD ls Prop) -> Prop with
+      | nil => fun P => P HList.Hnil
+      | l :: ls => fun P => exists x : typD l,
+                              _exists ls (fun z => P (HList.Hcons x z))
+    end.
+
+  Fixpoint _impls (ls : list Prop) (P : Prop) :=
+    match ls with
+      | nil => P
+      | l :: ls => l -> _impls ls P
+    end.
+
+  Section _and.
+    Context {A B : Type}.
+    Variables (a : A) (b : B).
+    Fixpoint _and (ls : list (A -> B -> Prop)) :=
+      match ls with
+        | nil => True
+        | l :: nil => l a b
+        | l :: ls => l a b /\ _and ls
+      end.
+  End _and.
+
+  Lemma _impls_sem
+  : forall ls P,
+      _impls ls P <-> (Forall (fun x => x) ls -> P).
+  Proof.
+    induction ls; simpl; intros.
+    + intuition.
+    + rewrite IHls. intuition.
+      inversion H0. eapply H; eauto.
+  Qed.
+  Lemma _exists_iff
+  : forall ls P Q,
+      (forall x, P x <-> Q x) ->
+      (@_exists ls P <-> @_exists ls Q).
+  Proof.
+    clear.
+    induction ls; simpl; intros.
+    + eapply H.
+    + apply exists_iff; intro. eapply IHls.
+      intro; eapply H.
+  Qed.
+  Lemma _forall_iff
+  : forall ls P Q,
+      (forall x, P x <-> Q x) ->
+      (@_foralls ls P <-> @_foralls ls Q).
+  Proof.
+    clear.
+    induction ls; simpl; intros.
+    + eapply H.
+    + apply forall_iff; intro. eapply IHls.
+      intro; eapply H.
+  Qed.
+
+  Lemma _exists_sem
+  : forall ls P,
+      _exists ls P <-> exists x, P x.
+  Proof.
+    clear. induction ls; simpl; auto.
+    - intuition. exists HList.Hnil. auto.
+      destruct H. rewrite (HList.hlist_eta x) in H.
+      assumption.
+    - intros. split.
+      + destruct 1.
+        eapply IHls in H.
+        destruct H. eauto.
+      + destruct 1.
+        exists (HList.hlist_hd x).
+        eapply IHls.
+        exists (HList.hlist_tl x).
+        rewrite (HList.hlist_eta x) in H.
+        assumption.
+  Qed.
+  Lemma _forall_sem
+  : forall ls P,
+      _foralls ls P <-> forall x, P x.
+  Proof.
+    clear. induction ls; simpl; auto.
+    - intuition. rewrite (HList.hlist_eta x).
+      assumption.
+    - intros. split.
+      + intros.
+        rewrite (HList.hlist_eta x).
+        eapply IHls in H.
+        eapply H.
+      + intros.
+        eapply IHls.
+        intros. eapply H.
+  Qed.
+End quants.
