theories/VariablesI.v
@@ -1,0 +1,79 @@
+Require Import Coq.Lists.List.
+Require Import ExtLib.Data.HList.
+Require Import MirrorCore.TypesI.
+Require Import MirrorCore.ExprI.
+Require Import MirrorCore.EnvI.
+
+Set Implicit Arguments.
+Set Strict Implicit.
+
+Section with_Expr.
+  Variable typ : Type.
+  Variable RType_typ : RType typ.
+  Variable expr : Type.
+  Variable Expr_expr : @Expr typ _ expr.
+
+  Class ExprVar : Type :=
+  { Var : nat -> expr
+  ; mentionsV : nat -> expr -> bool
+  }.
+
+  Class ExprVarOk (EV : ExprVar) : Prop :=
+  { Var_exprD'
+    : forall tus tvs v t,
+        match exprD' tus tvs (Var v) t with
+          | None =>
+            nth_error tvs v = None \/
+            exists t', nth_error tvs v = Some t' /\ ~Rty t t'
+          | Some vD =>
+            exists get,
+            nth_error_get_hlist_nth typD tvs v = Some (@existT _ _ t get) /\
+            forall us vs,
+              get vs = vD us vs
+        end
+  ; exprD'_strengthenV_single
+    : forall tus tvs e t t' val,
+      mentionsV (length tvs) e = false ->
+      exprD' tus (tvs ++ t :: nil) e t' = Some val ->
+      exists val',
+        exprD' tus tvs e t' = Some val' /\
+        forall us vs u,
+          val us (hlist_app vs (Hcons u Hnil)) = val' us vs
+  ; mentionsV_Var : forall v v', mentionsV v (Var v') = true <-> v = v'
+  }.
+
+  Class ExprUVar : Type :=
+  { UVar : nat -> expr
+  ; mentionsU : nat -> expr -> bool
+  }.
+
+  Class ExprUVarOk (EU : ExprUVar) : Prop :=
+  { UVar_exprD'
+    : forall tus tvs v t,
+        match exprD' tus tvs (UVar v) t with
+          | None =>
+            nth_error tvs v = None \/
+            exists t', nth_error tvs v = Some t' /\ ~Rty t t'
+          | Some vD =>
+            exists get,
+            nth_error_get_hlist_nth typD tvs v = Some (@existT _ _ t get) /\
+            forall us vs,
+              get vs = vD us vs
+        end
+  ; exprD'_strengthenU_single
+    : forall tus tvs e t t' val,
+      mentionsU (length tus) e = false ->
+      exprD' (tus ++ t :: nil) tvs e t' = Some val ->
+      exists val',
+        exprD' tus tvs e t' = Some val' /\
+        forall us vs u,
+          val (hlist_app us (Hcons u Hnil)) vs = val' us vs
+  ; mentionsU_UVar : forall v v', mentionsU v (UVar v') = true <-> v = v'
+  }.
+
+End with_Expr.
+
+Arguments ExprVar expr : rename.
+Arguments ExprUVar expr : rename.
+Arguments ExprVarOk {typ _ expr _} _ : rename.
+Arguments ExprUVarOk {typ _ expr _} _ : rename.
